words

Semantics.v
@@ -1,61 +1,174 @@
 Set Implicit Arguments.
 
 Require Import Syntax.
-Require Import Coq.Sets.Ensembles.
+Require Import Coq.Classes.Equivalence.
 Require Import Coq.Arith.EqNat.
+Require Import Coq.Logic.FunctionalExtensionality.
+Require Import Coq.Setoids.Setoid.
 
-Definition get_Field (pkt : packet) (fld : field) : nat :=
-  match fld with
-    | Src => pktSrc pkt
-    | Dst => pktDst pkt
-  end.
+Module Relation.
 
-Definition set_field (h : history) (fld : field) (n : nat) : history :=
-  match h with
-    | OneHist p => match fld with
-             | Src => OneHist (Packet n (get_Field p Dst))
-             | Dst => OneHist (Packet (get_Field p Src) n)
-             end
-    | ConsHist p hst => match fld with
-                  | Src => ConsHist (Packet n (get_Field p Dst)) hst
-                  | Dst => ConsHist (Packet (get_Field p Src) n) hst
-                  end
+  Section Defs.
+
+    Variable A : Type.
+    
+    Definition relation := A -> A -> Prop.
+    
+    Definition union (R1 R2 : relation) : relation :=
+      fun (x y : A) => R1 x y \/ R2 x y.
+    
+    Definition join (R1 R2 : relation) : relation :=
+      fun (x y : A) => exists (z : A), R1 x z /\ R2 z y.
+    
+    Definition empty : relation :=
+      fun (x y : A) => False.
+    
+    Definition id : relation :=
+      fun (x y : A) => x = y.
+    
+    Fixpoint expt (R : relation) (n : nat) : relation :=
+      match n with
+        | 0 => id
+        | S m => join R (expt R m)
+      end.
+    
+    Definition star (R : relation) : relation :=
+      fun (x y : A) => exists n, (expt R n) x y.
+
+    Definition inv (R : relation) : relation :=
+      fun (x y : A) => R x y -> False /\ (R x y -> False) -> True.
+
+    Definition equiv (R1 R2 : relation) :=
+      forall (x y : A), R1 x y <-> R2 x y.
+
+  End Defs.
+
+  Instance Equivalence_equiv `(A : Type) : Equivalence (@equiv A).
+  Proof with auto.
+    split; unfold equiv.
+    + unfold Reflexive.
+      intros. intuition.
+    + unfold Symmetric.
+      intros. symmetry. apply H.
+    + unfold Transitive.
+      intros.
+      split... 
+      - intros.
+        apply H0.
+        apply H...
+      - intros.
+        apply H.
+        apply H0...
+  Qed.
+
+End Relation.
+
+Module Semantics.
+
+  Import Relation.
+
+  Definition get_Field (pkt : packet) (fld : field) : nat :=
+    match fld with
+      | Src => pktSrc pkt
+      | Dst => pktDst pkt
+    end.
+
+  Definition set_field (h : history) (fld : field) (n : nat) : history :=
+    match h with
+      | OneHist p => match fld with
+                       | Src => OneHist (Packet n (get_Field p Dst))
+                       | Dst => OneHist (Packet (get_Field p Src) n)
+                     end
+      | ConsHist p hst => match fld with
+                            | Src => ConsHist (Packet n (get_Field p Dst)) hst
+                            | Dst => ConsHist (Packet (get_Field p Src) n) hst
+                          end
     end.        
 
-Definition get_Packet (hst : history) : packet :=
-  match hst with
-    | OneHist p => p
-    | ConsHist p h => p
-  end.
+  Definition get_Packet (hst : history) : packet :=
+    match hst with
+      | OneHist p => p
+      | ConsHist p h => p
+    end.
 
-Definition Kleisli {A : Type} (rel1 rel2 : A -> A -> Prop) (ina outa : A) : Prop :=
-  exists (x : A), (rel1 ina x) /\ (rel2 x outa).
+  Locate exp.
+  Check exp.
+  Check relation.
+  Fixpoint eval (e : exp) : relation history :=
+    match e with
+      | Drop => @empty history
+      | Id => @id history
+      | Match f v => 
+        fun (h r : history) =>
+          match beq_nat (get_Field (get_Packet h) f) v with 
+            | true => h = r
+            | false => False
+          end
+      | Mod f v => 
+        fun (h r : history) => r = set_field h f v
+      | Par e1 e2 => union (eval e1) (eval e2)
+      | Neg e1 => inv (eval e1)
+      | Obs => fun (h r : history) => r= (ConsHist (get_Packet h) h)
+      | Seq e1 e2 => join (eval e1) (eval e2)
+      | Star e1 => star (eval e1)
+    end.
 
-Check Singleton.
+  Definition equiv_exp (e1 : exp) (e2 : exp) : Prop := 
+    equiv (eval e1) (eval e2).
 
-Check In_singleton.
-Fixpoint iter (rel : history -> history -> Prop) (i : nat) (inh : history) : Ensemble history :=
-  match i with
-   | O => Singleton history inh
-   | S n => (Kleisli rel (iter rel (n))) inh
-  end.
+  Instance Equivalence_exp : Equivalence equiv_exp.
+  Proof with auto.
+    unfold equiv_exp.
+    split.
+    + unfold Reflexive.
+      intros.
+      apply reflexivity.
+    + unfold Symmetric.
+      intros.
+      apply symmetry...
+    + unfold Transitive.
+      intros.
+      eapply transitivity; eauto.
+  Qed.
 
-Fixpoint eval (e : exp) (h : history) : Ensemble history :=
-  match e with
-   | Drop => @Empty_set history
-   | Id => Singleton _ h
-   | Match f v => match beq_nat (get_Field (get_Packet h) f) v with 
-                    | true => Singleton _ h
-                    | false => @Empty_set history
-                  end
-   | Mod f v => Singleton _ (set_field h f v)
-   | Par e1 e2 => Union _ (eval e1 h) (eval e2 h)
-   | Neg e1 => Setminus _ (Singleton _ h) (eval e1 h)
-   | Obs => Singleton _ (ConsHist (get_Packet h) h)
-   | Seq e1 e2 => Kleisli (eval e1) (eval e2) h
-   | Star e1 => fun (y : history) => exists (i : nat), (iter (eval e1) i h y)
-  end.
+End Semantics.
 
-Definition equiv_exp (e1 : exp) (e2 : exp) : Prop := 
-  forall (h : history),  (eval e1 h) = (eval e2 h).
- 
+Module BooleanAlgebra.
+
+  Import Semantics.
+  Import Syntax.
+  Import Relation.
+
+  Existing Instances Equivalence_exp.
+  Local Open Scope equiv_scope.
+
+
+  (* Predicates are either identity or empty *)
+  Lemma bool_spec : forall (e : exp),
+    pred e ->
+    forall (h r : history),
+      eval e h r -> (False \/ h = r).
+  Proof with auto.
+    intros.
+    induction H...
+  Admitted.
+
+  Lemma BA_Plus_One : 
+    forall (e : exp),
+      pred e ->
+      (Par e Id) === Id.
+  Proof with auto.
+    intros.
+    split.
+    + intros. simpl in *. 
+      unfold union in H0.
+      destruct H0...
+      destruct (bool_spec H x y H0)...
+      contradiction.
+    + intros.
+      simpl in *.
+      unfold union...
+  Qed.
+
+  Lemma BA_Excl_Mid : 
+    
